Invariance.v
@@ -1,0 +1,4 @@
+Fixpoint filterList {X:Type} (l1 l2:list X) (cmp:X->X->bool) : list X :=
+  match l1 with
+  | nil => nil
+  | cons x xrem => 
