Progress.v
@@ -12,15 +12,102 @@ forall (st:DVMState) (p:Program) (i:Instruction), consistentInst i st p ->
 
 *)
 
-(*
-Theorem pregress : forall (st:DVMState) (p:Program) (i:Instruction), consistentInst i st p -> 
+Theorem progressReg : forall (x:Register) (frms:list Frame) (h:Heap) (sh:SHeap) (inb outb:Buffer), consistentEvalReg x (dst frms h sh inb outb) ->
+  isNone (EVAL.evalReg x (dst frms h sh inb outb)) = false.
+Proof.
+  intros. inversion H. unfold EVAL.evalReg. destruct x; apply EVAL.RLIST.findRelEq in H2; rewrite H2; simpl.
+  assert (exists v,EVAL.RLIST.get n' vals = Some v).
+    eapply EVAL.RLIST.get_find. apply H2.
+    inversion H7. rewrite H8. destruct x. simpl. reflexivity.
+    apply EVAL.RLIST.get_find in H2. inversion H2. rewrite H7. destruct x0. simpl. reflexivity.
+  Qed.
+
+Theorem progressLhs : forall (x:lhs) (frms:list Frame) (h:Heap) (sh:SHeap) (inb outb:Buffer), consistentEvalLhs x (dst frms h sh inb outb) ->
+  isNone (EVAL.evalLhs x (dst frms h sh inb outb)) = false.
+Proof.
+  intros. inversion H.
+    simpl. apply progressReg. assumption.
+    simpl. apply EVAL.evalRegRelEq in H5. apply EVAL.evalRegRelEq in H8.
+    rewrite H5. apply EVAL.HP.getRelEq in H7. rewrite H7. rewrite H8. rewrite <- H9 in H11. eapply EVAL.VLIST.get_avail in H11.
+    apply PType.toNatRelEq in H10. rewrite H10. inversion H11. rewrite H12. reflexivity.
+    assert (exists v', EVAL.evalLhs (ifield n n2) (dst frms h sh inb outb) = Some v').
+      remember (EVAL.evalLhs (ifield n n2) (dst frms h sh inb outb)) as tmp.
+        destruct vl. exists v. rewrite Heqtmp.
+        eapply EVAL.evalLhsRelEq. econstructor; try eassumption.
+    inversion H10. rewrite H11. simpl. reflexivity.
+    assert (exists v', EVAL.evalLhs (sfield n) (dst frms h sh inb outb) = Some v').
+      destruct vl. exists v. apply EVAL.evalLhsRelEq. econstructor.
+        apply H3. apply H7. inversion H8. rewrite H9.
+    reflexivity.
+  Qed.
+
+Theorem progressRhs : forall (x:rhs) (frms:list Frame) (h:Heap) (sh:SHeap) (inb outb:Buffer), consistentEvalRhs x (dst frms h sh inb outb) ->
+  isNone (EVAL.evalRhs x (dst frms h sh inb outb)) = false.
+Proof.
+  intros. inversion H. simpl. apply progressLhs. assumption.
+  simpl. destruct cns; reflexivity.
+  Qed.
+
+Theorem progress : forall (st:DVMState) (p:Program) (i:Instruction), consistentInst i st p -> 
   (exists st',INSTRUCTION.stepWith i st p = Some st' /\ ~(st' = stuck)).
 Proof.
   destruct st.
     intros p i.
     generalize dependent p.
     destruct i; intros; inversion H.
+    (** nop *)
       inversion H0; simpl; eapply ex_intro. split. unfold INSTRUCTION.stepWith.
         unfold INSTRUCTION.evalInst. simpl. rewrite H9. rewrite H10. reflexivity.
         intro. inversion H11.
-*)
+    (** ret *)
+      inversion H0; simpl. unfold INSTRUCTION.stepWith.
+        unfold INSTRUCTION.evalInst. unfold INSTRUCTION.evalRet. rewrite H9. rewrite H10.
+        destruct (EVAL.evalReg 201 (dst (f :: frm vals ml pc :: frms0) h sh inb outb)); simpl.
+          destruct (ChangeState.VLIST.find (201, v) compFirst vals). simpl.
+          exists (dst (frm (ChangeState.VLIST.set n (201, v) vals) ml pc' :: frms0) h sh inb outb).
+          split. reflexivity. intro. inversion H11.
+          exists (dst (ChangeState.changeFrame (frm (ChangeState.VLIST.prep (201, v) vals) ml pc) (upPC pc') :: frms0) h sh inb outb).
+          split. reflexivity. intro. inversion H11.
+          exists (dst (frm vals ml pc' :: frms0) h sh inb outb).
+          split. reflexivity. intro. inversion H11.
+    (** retTo *)
+      inversion H1; simpl. unfold INSTRUCTION.stepWith.
+        unfold INSTRUCTION.evalInst. unfold INSTRUCTION.evalRetTo. rewrite H10. rewrite H11.
+        destruct (EVAL.evalReg 201 (dst (f :: frm vals ml pc :: frms0) h sh inb outb)); simpl.
+          destruct (ChangeState.VLIST.find (201, v) compFirst vals). simpl.
+          exists (dst (ChangeState.changeFrame
+                      match ChangeState.VLIST.find (r, v) compFirst vals with
+                      | Some n' => frm (ChangeState.VLIST.set n' (r, v) vals) ml pc
+                      | None => frm (ChangeState.VLIST.prep (r, v) vals) ml pc
+                      end (upPC pc') :: frms0) h sh inb outb).
+          split. reflexivity. intro. inversion H12.
+          exists (dst (ChangeState.changeFrame
+                      match ChangeState.VLIST.find (r, v) compFirst vals with
+                      | Some n' => frm (ChangeState.VLIST.set n' (r, v) vals) ml pc
+                      | None => frm (ChangeState.VLIST.prep (r, v) vals) ml pc
+                      end (upPC pc') :: frms0) h sh inb outb).
+          split. reflexivity. intro. inversion H12.
+          exists (dst (frm vals ml pc' :: frms0) h sh inb outb).
+          split. reflexivity. intro. inversion H12.
+    (** invokes *)
+      inversion H4. unfold INSTRUCTION.stepWith.
+        unfold INSTRUCTION.evalInst. unfold INSTRUCTION.evalInvokes.
+        assert ((filter (map l (fun x : rhs => EVAL.evalRhs x (dst frms h sh inb outb))) isNone) = []).
+        eapply forAllListFilter.
+        assert (forall x : rhs, (fun y:rhs => consistentEvalRhs y (dst frms h sh inb outb)) x -> isNone (EVAL.evalRhs x (dst frms h sh inb outb)) = false).
+          intros. apply progressRhs; try eassumption. eassumption. assumption.
+        rewrite H15. rewrite H13. simpl.
+        (** Resolve Here *)
+              destruct (fastRev
+       (List.map
+          (fun x : nat * Val =>
+           let (nx, vx) := x in updateFrame (upVals nx vx))
+          (numberList 101
+             (List.map
+                (fun x : rhs =>
+                 match EVAL.evalRhs x (dst frms h sh inb outb) with
+                 | Some v1 => v1
+                 | None => ref null
+                 end) (fastRev l))))). eexists. split. reflexivity.
+          intro Contra. inversion Contra.
+          simpl. unfold fastRev. simpl.
